fstar/MLS.TreeSync.IntegrityCheck.fst
@@ -42,18 +42,21 @@ let integrity_either_to_bool ie =
   | IE_Good -> true
   | _ -> false
 
-val check_signature: #bytes:Type0 -> {|crypto_bytes bytes|} -> #tkt:treekem_types bytes -> leaf_node_nt bytes tkt -> bytes -> result (option leaf_integrity_error)
-let check_signature #bytes #cb #tkt lp group_id =
+val check_signature: #bytes:Type0 -> {|crypto_bytes bytes|} -> #tkt:treekem_types bytes -> leaf_node_nt bytes tkt -> bytes -> nat -> result (option leaf_integrity_error)
+let check_signature #bytes #cb #tkt lp group_id leaf_index =
   if not (length #bytes lp.data.signature_key = sign_public_key_length #bytes) then
     error "check_leaf_package: signature key has wrong length"
   else if not (length #bytes lp.signature = sign_signature_length #bytes) then
     error "check_leaf_package: signature has wrong length"
   else if not (length group_id < pow2 30) then
     error "check_leaf_package: group_id too long"
+  else if not (leaf_index < pow2 32) then
+    error "check_leaf_package: leaf_index too big"
   else (
     let tbs = ({
       data = lp.data;
       group_id = (match lp.data.source with | LNS_commit () | LNS_update () -> group_id | _ -> ());
+      leaf_index = (match lp.data.source with | LNS_commit () | LNS_update () -> leaf_index | _ -> ());
     } <: leaf_node_tbs_nt bytes tkt) in
     let leaf_package_bytes: bytes = serialize (leaf_node_tbs_nt bytes _) tbs in
     if not (length leaf_package_bytes < pow2 30 && sign_with_label_pre #bytes "LeafNodeTBS" (length #bytes leaf_package_bytes)) then error "check_signature: tbs too long"
@@ -92,7 +95,7 @@ let check_leaf #bytes #cb leaf_index olp group_id =
   match olp with
   | None -> return IE_Good
   | Some lp -> (
-    signature_check <-- check_signature lp group_id;
+    signature_check <-- check_signature lp group_id leaf_index;
     capabilities_check <-- check_capabilities lp;
     lifetime_check <-- check_lifetime lp;
     let signature_either = convert_opt_leaf_error_to_either signature_check leaf_index in
